refactor: standardize predicate naming to lowercase

avl.dfy
@@ -7,30 +7,30 @@ class AvlNode {
   var left: AvlNode?
   var right: AvlNode?
 
-  ghost predicate Height_Valid()
+  ghost predicate height_valid()
     reads this, Repr
   {
     this in Repr &&
     (left != null ==> left in Repr && left.Repr <= Repr && this !in left.Repr) &&
     (right != null ==> right in Repr && right.Repr <= Repr && this !in right.Repr) &&
     (left != null && right != null ==> left.Repr !! right.Repr) &&
-    (left != null ==> left.Height_Valid()) &&
-    (right != null ==> right.Height_Valid()) &&
+    (left != null ==> left.height_valid()) &&
+    (right != null ==> right.height_valid()) &&
     height == 1 + max(if left == null then -1 else left.height, if right == null then -1 else right.height)
   }
 
   // difference in subtree heights ≤ 1
-  ghost predicate Balanced()
+  ghost predicate balanced()
     reads this, Repr
   {
     this in Repr &&
-    Height_Valid() &&
-    Valid() &&
-    (left != null ==> left in Repr && left.Balanced()) &&
-    (right != null ==> right in Repr && right.Balanced()) &&
-    var leftHeight := if left == null then -1 else left.height;
-    var rightHeight := if right == null then -1 else right.height;
-    leftHeight - rightHeight <= 1 && rightHeight - leftHeight <= 1
+    height_valid() &&
+    valid() &&
+    (left != null ==> left in Repr && left.balanced()) &&
+    (right != null ==> right in Repr && right.balanced()) &&
+    var leftheight := if left == null then -1 else left.height;
+    var rightheight := if right == null then -1 else right.height;
+    leftheight - rightheight <= 1 && rightheight - leftheight <= 1
   }
 
   function max(a: int, b: int) : int
@@ -38,24 +38,24 @@ class AvlNode {
     if a >= b then a else b
   }
 
-  ghost predicate Valid()
+  ghost predicate valid()
     reads this, Repr
   {
     this in Repr &&
     (left != null ==> left in Repr && left.Repr <= Repr && this !in left.Repr) &&
     (right != null ==> right in Repr && right.Repr <= Repr && this !in right.Repr) &&
     (left != null && right != null ==> left.Repr !! right.Repr) &&
-    (left != null ==> left.Valid()) &&
-    (right != null ==> right.Valid()) &&
+    (left != null ==> left.valid()) &&
+    (right != null ==> right.valid()) &&
     Contents == {data} + (if left == null then {} else left.Contents) + (if right == null then {} else right.Contents) &&
     Repr == {this} + (if left == null then {} else left.Repr) + (if right == null then {} else right.Repr)
   }
 
   // init leaf node with value x
   constructor Init(x: int)
-    ensures Valid() && fresh(Repr - {this})
-    ensures Height_Valid()
-    ensures Balanced()
+    ensures valid() && fresh(Repr - {this})
+    ensures height_valid()
+    ensures balanced()
     ensures Contents == {x}
     ensures Repr == {this}
   {
@@ -74,7 +74,7 @@ class AvlTree {
 
   var root: AvlNode?;
 
-  ghost predicate Valid()
+  ghost predicate valid()
     reads this, root, if root != null then root.Repr else {}
   {
     // empty
@@ -82,24 +82,24 @@ class AvlTree {
       Contents == {}
     else
       root in Repr && root.Repr <= Repr &&
-      root.Valid() &&
+      root.valid() &&
       Contents == root.Contents
   }
 
-  ghost predicate Balanced()
+  ghost predicate balanced()
     reads this, root, if root != null then root.Repr else {}
   {
     if root == null then
       true
     else
-      root.Balanced()
+      root.balanced()
   }
 
   // init empty AVL tree
   constructor Init()
-    ensures Valid() && fresh(Repr - {this})
+    ensures valid() && fresh(Repr - {this})
     ensures Contents == {}
-    ensures Balanced()
+    ensures balanced()
   {
     root := null;
     Repr := {this};
